#discretemath 
| Equivalence | Name |
|-|-|
|¬(p∧q)≡¬p∨¬q, ¬(p∨q)≡¬p∧¬q|DeMorgan's Laws |
| p ∧ T ≡ p,<br/> p ∨ F ≡ p | Identity Laws |
| p ∨ T ≡ T,<br/> p ∧ F ≡ F | Domination Laws |
| p ∨ p ≡ p,<br/> p ∧ p ≡ p | Idempotent Laws |
|¬(¬p) ≡ p |Double negation law|
|p ∨ q ≡ q ∨ p,<br/> p ∧ q ≡ q ∧ p|Commutative Laws |
|(p ∨ q) ∨ r ≡ p ∨ (q ∨ r),<br/> (p ∧ q) ∧ r ≡ p ∧ (q ∧ r)|Associative Laws |
|p ∨ (q ∧ r) ≡ (p ∨ q) ∧ (p ∨ r),<br/> p ∧ (q ∨ r) ≡ (p ∧ q) ∨ (p ∧ r)|Distributive Laws|
|p ∨ (p ∧ q) ≡ p, <br/>  p ∧ (p ∨ q) ≡ p| Absorption Laws |
|p ∨ ¬p ≡ T, <br/> p ∧ ¬p ≡ F| Negation Laws |

Logical Equivalences Involving Conditional Statements:
p → q ≡ ¬p ∨ q  
p → q ≡ ¬q → ¬p  
p ∨ q ≡ ¬p → q  
p ∧ q ≡ ¬(p → ¬q)  
¬(p → q) ≡ p ∧ ¬q  
(p → q) ∧ (p → r) ≡ p → (q ∧ r)  
(p → r) ∧ (q → r) ≡ (p ∨ q) → r  
(p → q) ∨ (p → r) ≡ p → (q ∨ r)  
(p → r) ∨ (q → r) ≡ (p ∧ q) → r

Logical Equivalences Involving Biconditional Statements:
p ↔ q ≡ (p → q) ∧ (q → p)  
p ↔ q ≡ ¬p ↔ ¬q  
p ↔ q ≡ (p ∧ q) ∨ (¬p ∧ ¬q)  
¬(p ↔ q) ≡ p ↔ ¬q